Test/dafny1/SchorrWaite.dfy
@@ -7,10 +7,10 @@
 // Copyright (c) 2008, Microsoft.
 
 class Node {
-  var children: seq<Node>;
-  var marked: bool;
-  var childrenVisited: int;
-  ghost var pathFromRoot: Path;
+  var children: seq<Node>
+  var marked: bool
+  var childrenVisited: int
+  ghost var pathFromRoot: Path
 }
 
 datatype Path = Empty | Extend(Path, Node)
@@ -18,61 +18,61 @@ datatype Path = Empty | Extend(Path, Node)
 
 class Main {
   method RecursiveMark(root: Node, ghost S: set<Node>)
-    requires root in S;
+    requires root in S
     // S is closed under 'children':
-    requires (forall n :: n in S ==> n != null &&
-                (forall ch :: ch in n.children ==> ch == null || ch in S));
-    requires (forall n :: n in S ==> ! n.marked && n.childrenVisited == 0);
-    modifies S;
-    ensures root.marked;
+    requires forall n :: n in S ==> n != null &&
+                forall ch :: ch in n.children ==> ch == null || ch in S
+    requires forall n :: n in S ==> !n.marked && n.childrenVisited == 0
+    modifies S
+    ensures root.marked
     // nodes reachable from 'root' are marked:
-    ensures (forall n :: n in S && n.marked ==>
-                (forall ch :: ch in n.children && ch != null ==> ch.marked));
-    ensures (forall n :: n in S ==>
+    ensures forall n :: n in S && n.marked ==>
+                forall ch :: ch in n.children && ch != null ==> ch.marked
+    ensures forall n :: n in S ==>
                 n.childrenVisited == old(n.childrenVisited) &&
-                n.children == old(n.children));
+                n.children == old(n.children)
   {
     RecursiveMarkWorker(root, S, {});
   }
 
   method RecursiveMarkWorker(root: Node, ghost S: set<Node>, ghost stackNodes: set<Node>)
-    requires root != null && root in S;
-    requires (forall n :: n in S ==> n != null &&
-                (forall ch :: ch in n.children ==> ch == null || ch in S));
-    requires (forall n :: n in S && n.marked ==>
+    requires root != null && root in S
+    requires forall n :: n in S ==> n != null &&
+                forall ch :: ch in n.children ==> ch == null || ch in S
+    requires forall n :: n in S && n.marked ==>
                 n in stackNodes ||
-                (forall ch :: ch in n.children && ch != null ==> ch.marked));
-    requires (forall n :: n in stackNodes ==> n != null && n.marked);
-    modifies S;
-    ensures root.marked;
+                forall ch :: ch in n.children && ch != null ==> ch.marked
+    requires forall n :: n in stackNodes ==> n != null && n.marked
+    modifies S
+    ensures root.marked
     // nodes reachable from 'root' are marked:
-    ensures (forall n :: n in S && n.marked ==>
+    ensures forall n :: n in S && n.marked ==>
                 n in stackNodes ||
-                (forall ch :: ch in n.children && ch != null ==> ch.marked));
-    ensures (forall n: Node :: n in S && old(n.marked) ==> n.marked);
-    ensures (forall n :: n in S ==>
+                forall ch :: ch in n.children && ch != null ==> ch.marked
+    ensures forall n: Node :: n in S && old(n.marked) ==> n.marked
+    ensures forall n :: n in S ==>
                 n.childrenVisited == old(n.childrenVisited) &&
-                n.children == old(n.children));
-    decreases S - stackNodes;
+                n.children == old(n.children)
+    decreases S - stackNodes
   {
-    if (! root.marked) {
+    if !root.marked {
       root.marked := true;
       var i := 0;
-      while (i < |root.children|)
-        invariant root.marked && i <= |root.children|;
-        invariant (forall n :: n in S && n.marked ==>
+      while i < |root.children|
+        invariant root.marked && i <= |root.children|
+        invariant forall n :: n in S && n.marked ==>
                 n == root ||
                 n in stackNodes ||
-                (forall ch :: ch in n.children && ch != null ==> ch.marked));
-        invariant (forall j :: 0 <= j && j < i ==>
-                    root.children[j] == null || root.children[j].marked);
-        invariant (forall n: Node :: n in S && old(n.marked) ==> n.marked);
-        invariant (forall n :: n in S ==>
+                forall ch :: ch in n.children && ch != null ==> ch.marked
+        invariant forall j :: 0 <= j < i ==>
+                    root.children[j] == null || root.children[j].marked
+        invariant forall n: Node :: n in S && old(n.marked) ==> n.marked
+        invariant forall n :: n in S ==>
                 n.childrenVisited == old(n.childrenVisited) &&
-                n.children == old(n.children));
+                n.children == old(n.children)
       {
         var c := root.children[i];
-        if (c != null) {
+        if c != null {
           RecursiveMarkWorker(c, S, stackNodes + {root});
         }
         i := i + 1;
@@ -83,59 +83,59 @@ class Main {
   // ---------------------------------------------------------------------------------
 
   method IterativeMark(root: Node, ghost S: set<Node>)
-    requires root in S;
+    requires root in S
     // S is closed under 'children':
-    requires (forall n :: n in S ==> n != null &&
-                (forall ch :: ch in n.children ==> ch == null || ch in S));
-    requires (forall n :: n in S ==> ! n.marked && n.childrenVisited == 0);
-    modifies S;
-    ensures root.marked;
+    requires forall n :: n in S ==> n != null &&
+                forall ch :: ch in n.children ==> ch == null || ch in S
+    requires forall n :: n in S ==> !n.marked && n.childrenVisited == 0
+    modifies S
+    ensures root.marked
     // nodes reachable from 'root' are marked:
-    ensures (forall n :: n in S && n.marked ==>
-                (forall ch :: ch in n.children && ch != null ==> ch.marked));
-    ensures (forall n :: n in S ==>
+    ensures forall n :: n in S && n.marked ==>
+                forall ch :: ch in n.children && ch != null ==> ch.marked
+    ensures forall n :: n in S ==>
                 n.childrenVisited == old(n.childrenVisited) &&
-                n.children == old(n.children));
+                n.children == old(n.children)
   {
     var t := root;
     t.marked := true;
     var stackNodes := [];
     ghost var unmarkedNodes := S - {t};
-    while (true)
-      invariant root.marked && t in S && t !in stackNodes;
+    while true
+      invariant root.marked && t in S && t !in stackNodes
       // stackNodes has no duplicates:
-      invariant (forall i, j :: 0 <= i && i < j && j < |stackNodes| ==>
-                  stackNodes[i] != stackNodes[j]);
-      invariant (forall n :: n in stackNodes ==> n in S);
-      invariant (forall n :: n in stackNodes || n == t ==>
+      invariant forall i, j :: 0 <= i < j < |stackNodes| ==>
+                  stackNodes[i] != stackNodes[j]
+      invariant forall n :: n in stackNodes ==> n in S
+      invariant forall n :: n in stackNodes || n == t ==>
                   n.marked &&
-                  0 <= n.childrenVisited && n.childrenVisited <= |n.children| &&
-                  (forall j :: 0 <= j && j < n.childrenVisited ==>
-                    n.children[j] == null || n.children[j].marked));
-      invariant (forall n :: n in stackNodes ==> n.childrenVisited < |n.children|);
+                  0 <= n.childrenVisited <= |n.children| &&
+                  forall j :: 0 <= j < n.childrenVisited ==>
+                    n.children[j] == null || n.children[j].marked
+      invariant forall n :: n in stackNodes ==> n.childrenVisited < |n.children|
       // nodes on the stack are linked:
-      invariant (forall j :: 0 <= j && j+1 < |stackNodes| ==>
-                  stackNodes[j].children[stackNodes[j].childrenVisited] == stackNodes[j+1]);
+      invariant forall j :: 0 <= j && j+1 < |stackNodes| ==>
+                  stackNodes[j].children[stackNodes[j].childrenVisited] == stackNodes[j+1]
       invariant 0 < |stackNodes| ==>
-        stackNodes[|stackNodes|-1].children[stackNodes[|stackNodes|-1].childrenVisited] == t;
-      invariant (forall n :: n in S && n.marked && n !in stackNodes && n != t ==>
-                  (forall ch :: ch in n.children && ch != null ==> ch.marked));
-      invariant (forall n :: n in S && n !in stackNodes && n != t ==>
-                n.childrenVisited == old(n.childrenVisited));
-      invariant (forall n: Node :: n in S ==> n.children == old(n.children));
-      invariant (forall n :: n in S && !n.marked ==> n in unmarkedNodes);
-      decreases unmarkedNodes, stackNodes, |t.children| - t.childrenVisited;
+        stackNodes[|stackNodes|-1].children[stackNodes[|stackNodes|-1].childrenVisited] == t
+      invariant forall n :: n in S && n.marked && n !in stackNodes && n != t ==>
+                  forall ch :: ch in n.children && ch != null ==> ch.marked
+      invariant forall n :: n in S && n !in stackNodes && n != t ==>
+                  n.childrenVisited == old(n.childrenVisited)
+      invariant forall n: Node :: n in S ==> n.children == old(n.children)
+      invariant forall n :: n in S && !n.marked ==> n in unmarkedNodes
+      decreases unmarkedNodes, stackNodes, |t.children| - t.childrenVisited
     {
-      if (t.childrenVisited == |t.children|) {
+      if t.childrenVisited == |t.children| {
         // pop
         t.childrenVisited := 0;
-        if (|stackNodes| == 0) {
+        if |stackNodes| == 0 {
           return;
         }
         t := stackNodes[|stackNodes| - 1];
         stackNodes := stackNodes[..|stackNodes| - 1];
         t.childrenVisited := t.childrenVisited + 1;
-      } else if (t.children[t.childrenVisited] == null || t.children[t.childrenVisited].marked) {
+      } else if t.children[t.childrenVisited] == null || t.children[t.childrenVisited].marked {
         // just advance to next child
         t.childrenVisited := t.childrenVisited + 1;
       } else {
@@ -150,17 +150,17 @@ class Main {
 
   // ---------------------------------------------------------------------------------
 
-  function Reachable(from: Node, to: Node, S: set<Node>): bool
-    requires null !in S;
-    reads S;
+  predicate Reachable(from: Node, to: Node, S: set<Node>)
+    reads S
+    requires null !in S
   {
-    (exists via: Path :: ReachableVia(from, via, to, S))
+    exists via: Path :: ReachableVia(from, via, to, S)
   }
 
-  function ReachableVia(from: Node, via: Path, to: Node, S: set<Node>): bool
-    requires null !in S;
-    reads S;
-    decreases via;
+  predicate ReachableVia(from: Node, via: Path, to: Node, S: set<Node>)
+    reads S
+    requires null !in S
+    decreases via
   {
     match via
     case Empty => from == to
@@ -168,23 +168,23 @@ class Main {
   }
 
   method SchorrWaite(root: Node, ghost S: set<Node>)
-    requires root in S;
+    requires root in S
     // S is closed under 'children':
-    requires (forall n :: n in S ==> n != null &&
-                (forall ch :: ch in n.children ==> ch == null || ch in S));
+    requires forall n :: n in S ==> n != null &&
+                forall ch :: ch in n.children ==> ch == null || ch in S
     // the graph starts off with nothing marked and nothing being indicated as currently being visited:
-    requires (forall n :: n in S ==> ! n.marked && n.childrenVisited == 0);
-    modifies S;
+    requires forall n :: n in S ==> !n.marked && n.childrenVisited == 0
+    modifies S
     // nodes reachable from 'root' are marked:
-    ensures root.marked;
-    ensures (forall n :: n in S && n.marked ==>
-                (forall ch :: ch in n.children && ch != null ==> ch.marked));
+    ensures root.marked
+    ensures forall n :: n in S && n.marked ==>
+                forall ch :: ch in n.children && ch != null ==> ch.marked
     // every marked node was reachable from 'root' in the pre-state:
-    ensures (forall n :: n in S && n.marked ==> old(Reachable(root, n, S)));
+    ensures forall n :: n in S && n.marked ==> old(Reachable(root, n, S))
     // the structure of the graph has not changed:
-    ensures (forall n :: n in S ==>
+    ensures forall n :: n in S ==>
                 n.childrenVisited == old(n.childrenVisited) &&
-                n.children == old(n.children));
+                n.children == old(n.children)
   {
     var t := root;
     var p: Node := null;  // parent of t in original graph
@@ -193,52 +193,52 @@ class Main {
     t.pathFromRoot := path;
     ghost var stackNodes := [];
     ghost var unmarkedNodes := S - {t};
-    while (true)
-      invariant root.marked && t != null && t in S && t !in stackNodes;
-      invariant |stackNodes| == 0 <==> p == null;
-      invariant 0 < |stackNodes| ==> p == stackNodes[|stackNodes|-1];
+    while true
+      invariant root.marked && t != null && t in S && t !in stackNodes
+      invariant |stackNodes| == 0 <==> p == null
+      invariant 0 < |stackNodes| ==> p == stackNodes[|stackNodes|-1]
       // stackNodes has no duplicates:
-      invariant (forall i, j :: 0 <= i && i < j && j < |stackNodes| ==>
-                  stackNodes[i] != stackNodes[j]);
-      invariant (forall n :: n in stackNodes ==> n in S);
-      invariant (forall n :: n in stackNodes || n == t ==>
+      invariant forall i, j :: 0 <= i < j < |stackNodes| ==>
+                  stackNodes[i] != stackNodes[j]
+      invariant forall n :: n in stackNodes ==> n in S
+      invariant forall n :: n in stackNodes || n == t ==>
                   n.marked &&
-                  0 <= n.childrenVisited && n.childrenVisited <= |n.children| &&
-                  (forall j :: 0 <= j && j < n.childrenVisited ==>
-                    n.children[j] == null || n.children[j].marked));
-      invariant (forall n :: n in stackNodes ==> n.childrenVisited < |n.children|);
-      invariant (forall n :: n in S && n.marked && n !in stackNodes && n != t ==>
-                  (forall ch :: ch in n.children && ch != null ==> ch.marked));
-      invariant (forall n :: n in S && n !in stackNodes && n != t ==>
-                n.childrenVisited == old(n.childrenVisited));
-      invariant (forall n :: n in S ==> n in stackNodes || n.children == old(n.children));
-      invariant (forall n :: n in stackNodes ==>
+                  0 <= n.childrenVisited <= |n.children| &&
+                  forall j :: 0 <= j < n.childrenVisited ==>
+                    n.children[j] == null || n.children[j].marked
+      invariant forall n :: n in stackNodes ==> n.childrenVisited < |n.children|
+      invariant forall n :: n in S && n.marked && n !in stackNodes && n != t ==>
+                  forall ch :: ch in n.children && ch != null ==> ch.marked
+      invariant forall n :: n in S && n !in stackNodes && n != t ==>
+                  n.childrenVisited == old(n.childrenVisited)
+      invariant forall n :: n in S ==> n in stackNodes || n.children == old(n.children)
+      invariant forall n :: n in stackNodes ==>
                   |n.children| == old(|n.children|) &&
-                  (forall j :: 0 <= j && j < |n.children| ==>
-                    j == n.childrenVisited || n.children[j] == old(n.children[j])));
+                  forall j :: 0 <= j < |n.children| ==>
+                    j == n.childrenVisited || n.children[j] == old(n.children[j])
       // every marked node is reachable:
       invariant !fresh(path);  // needed to show 'path' worthy as argument to old(Reachable(...))
       invariant old(ReachableVia(root, path, t, S));
-      invariant (forall n, pth :: n in S && n.marked && pth == n.pathFromRoot ==> !fresh(pth));
-      invariant (forall n, pth :: n in S && n.marked && pth == n.pathFromRoot ==>
-                  old(ReachableVia(root, pth, n, S)));
-      invariant (forall n :: n in S && n.marked ==> old(Reachable(root, n, S)));
+      invariant forall n, pth :: n in S && n.marked && pth == n.pathFromRoot ==> !fresh(pth)
+      invariant forall n, pth :: n in S && n.marked && pth == n.pathFromRoot ==>
+                  old(ReachableVia(root, pth, n, S))
+      invariant forall n :: n in S && n.marked ==> old(Reachable(root, n, S))
       // the current values of m.children[m.childrenVisited] for m's on the stack:
-      invariant 0 < |stackNodes| ==> stackNodes[0].children[stackNodes[0].childrenVisited] == null;
-      invariant (forall k :: 0 < k && k < |stackNodes| ==>
-                  stackNodes[k].children[stackNodes[k].childrenVisited] == stackNodes[k-1]);
+      invariant 0 < |stackNodes| ==> stackNodes[0].children[stackNodes[0].childrenVisited] == null
+      invariant forall k :: 0 < k < |stackNodes| ==>
+                  stackNodes[k].children[stackNodes[k].childrenVisited] == stackNodes[k-1]
       // the original values of m.children[m.childrenVisited] for m's on the stack:
-      invariant (forall k :: 0 <= k && k+1 < |stackNodes| ==>
-                  old(stackNodes[k].children)[stackNodes[k].childrenVisited] == stackNodes[k+1]);
+      invariant forall k :: 0 <= k && k+1 < |stackNodes| ==>
+                  old(stackNodes[k].children)[stackNodes[k].childrenVisited] == stackNodes[k+1]
       invariant 0 < |stackNodes| ==>
-        old(stackNodes[|stackNodes|-1].children)[stackNodes[|stackNodes|-1].childrenVisited] == t;
-      invariant (forall n :: n in S && !n.marked ==> n in unmarkedNodes);
-      decreases unmarkedNodes, stackNodes, |t.children| - t.childrenVisited;
+        old(stackNodes[|stackNodes|-1].children)[stackNodes[|stackNodes|-1].childrenVisited] == t
+      invariant forall n :: n in S && !n.marked ==> n in unmarkedNodes
+      decreases unmarkedNodes, stackNodes, |t.children| - t.childrenVisited
     {
-      if (t.childrenVisited == |t.children|) {
+      if t.childrenVisited == |t.children| {
         // pop
         t.childrenVisited := 0;
-        if (p == null) {
+        if p == null {
           return;
         }
         var oldP := p.children[p.childrenVisited];
@@ -250,7 +250,7 @@ class Main {
         t.childrenVisited := t.childrenVisited + 1;
         path := t.pathFromRoot;
 
-      } else if (t.children[t.childrenVisited] == null || t.children[t.childrenVisited].marked) {
+      } else if t.children[t.childrenVisited] == null || t.children[t.childrenVisited].marked {
         // just advance to next child
         t.childrenVisited := t.childrenVisited + 1;
 
